Add contents of Ironclad Maps.i.dfy

Maps/Maps.dfy
@@ -1,13 +1,85 @@
 module Maps {
-  // converts a map to a sequence
-  function method {:opaque} convert_map_to_seq<T>(n:int, m:map<int, T>): seq<T>
-    requires n >= 0;
-    requires forall i {:trigger i in m} :: 0 <= i < n ==> i in m;
-    ensures |convert_map_to_seq(n, m)| == n;
-    ensures var s := convert_map_to_seq(n, m);
-    forall i {:trigger s[i]} :: 0 <= i < n ==> s[i] == m[i];
+  predicate is_equal<A(!new), B>(x: map<A, B>, y: map<A, B>)
+    ensures is_equal(x, y) ==> x == y
   {
-      if n == 0 then []
-      else convert_map_to_seq(n-1, m) + [m[n-1]]
+    (forall a :: a in x <==> a in y) && (forall a :: a in x ==> x[a] == y[a])
   }
-}
+
+  function method domain<U(!new), V>(m: map<U,V>): set<U>
+    ensures forall i :: i in domain(m) <==> i in m
+  {
+    set s | s in m
+  }
+
+  function union<U(!new), V>(m: map<U, V>, m': map<U, V>): map<U, V>
+    requires m.Keys !! m'.Keys
+    ensures forall i :: i in union(m, m') <==> i in m || i in m'
+    ensures forall i :: i in m ==> union(m, m')[i] == m[i]
+    ensures forall i :: i in m' ==> union(m, m')[i] == m'[i]
+  {
+    map i | i in (domain(m) + domain(m')) :: if i in m then m[i] else m'[i]
+  }
+
+  function method remove<U(!new), V(!new)>(m: map<U, V>, u: U) : map<U, V>
+    requires u in m
+    decreases |m|
+    ensures |remove(m, u)| == |m| - 1
+    ensures !(u in remove(m, u))
+    ensures forall u' :: u' in remove(m, u) <==> u' in m && u' != u
+  {
+    var m' := map u' | u' in m && u' != u :: m[u'];
+    lemma_map_remove_one(m, m', u);
+    m'
+  }
+
+  lemma lemma_map_size_is_domain_size<S(!new), T(!new)>(dom: set<S>,
+                                                        m: map<S, T>)
+    requires dom == domain(m)
+    ensures |m| == |dom|
+  {
+    if |m| == 0 {
+    } else {
+      var x :| x in m;
+      var m' := map y | y in m && y != x :: m[y];
+      var dom' := dom - {x};
+      lemma_map_size_is_domain_size(dom', m');
+      assert m == m'[x := m[x]];
+    }
+  }
+
+  lemma lemma_maps_decrease<S(!new), T(!new)>(before: map<S, T>,
+                                              after: map<S, T>,
+                                              item_removed: S)
+    requires item_removed in before
+    requires after == map s | s in before && s != item_removed :: before[s]
+    ensures |after| < |before|
+  {
+    var domain_before := set s | s in before;
+    var domain_after := set s | s in after;
+
+    lemma_map_size_is_domain_size(domain_before, before);
+    lemma_map_size_is_domain_size(domain_after, after);
+
+    if |after| == |before| {
+      assert |domain_before - domain_after| > 0;
+    } else if |after| > |before| {
+      assert |domain_after - domain_before| == 0;
+    }
+  }
+
+  lemma lemma_map_remove_one<S(!new), T(!new)>(before: map<S, T>,
+                                               after: map<S, T>,
+                                               item_removed: S)
+    requires item_removed in before
+    requires after == map s | s in before && s != item_removed :: before[s]
+    ensures |after| + 1 == |before|
+  {
+    var domain_before := domain(before);
+    var domain_after := domain(after);
+
+    lemma_map_size_is_domain_size(domain_before, before);
+    lemma_map_size_is_domain_size(domain_after, after);
+
+    assert domain_after + {item_removed} == domain_before;
+  }
+} 
